midterm: add stuff to file

midterm/midterm_simplifier.v
@@ -5,6 +5,130 @@
 
 (* ********** *)
 
+(* student name: Alan Matthew Anggara
+   e-mail address: alan.matthew@u.yale-nus.edu.sg
+   student ID number: A0207754B
+ *)
+
+(* student name: Kim Young Il
+   e-mail address: youngil.kim@u.yale-nus.edu.sg
+   student ID number: A0207809Y
+ *)
+
+(* student name: Vibilan Jayanth
+   e-mail address: vibilan@u.yale-nus.edu.sg
+   student ID number: A0242417L
+ *)
+
+(* ********** *)
+
+Ltac fold_unfold_tactic name := intros; unfold name; fold name; reflexivity.
+
+Require Import Arith Bool List.
+
+Inductive arithmetic_expression : Type :=
+  Literal : nat -> arithmetic_expression
+| Plus : arithmetic_expression -> arithmetic_expression -> arithmetic_expression
+| Times : arithmetic_expression -> arithmetic_expression -> arithmetic_expression.
+
+Fixpoint eqb_arithmetic_expression (ae1 ae2 : arithmetic_expression) : bool :=
+  match ae1 with
+  | Literal n1 =>
+      match ae2 with
+      | Literal n2 => Nat.eqb n1 n2
+      | _ => false
+      end
+  | Plus ae11 ae12 =>
+      match ae2 with
+      | Plus ae21 ae22 =>
+          eqb_arithmetic_expression ae11 ae21 && eqb_arithmetic_expression ae12 ae22
+      | _ => false
+      end
+  | Times ae11 ae12 =>
+      match ae2 with
+      | Times ae21 ae22 =>
+          eqb_arithmetic_expression ae11 ae21 && eqb_arithmetic_expression ae12 ae22
+      | _ => false
+      end
+  end.
+
+Inductive expressible_value : Type :=
+  Expressible_nat : nat -> expressible_value.
+
+Fixpoint evaluate_ltr (ae : arithmetic_expression) : expressible_value :=
+  match ae with
+  | Literal n =>
+    Expressible_nat n
+  | Plus e1 e2 =>
+    match evaluate_ltr e1 with
+    | Expressible_nat n1 =>
+      match evaluate_ltr e2 with
+      | Expressible_nat n2 =>
+        Expressible_nat (n1 + n2)
+      end
+    end
+  | Times e1 e2 =>
+    match evaluate_ltr e1 with
+    | Expressible_nat n1 =>
+      match evaluate_ltr e2 with
+      | Expressible_nat n2 =>
+        Expressible_nat (n1 * n2)
+      end
+    end
+  end.
+
+Lemma fold_unfold_evaluate_ltr_Literal :
+  forall n : nat,
+    evaluate_ltr (Literal n) =
+      Expressible_nat n.
+Proof.
+  fold_unfold_tactic evaluate_ltr.
+Qed.
+
+Lemma fold_unfold_evaluate_ltr_Plus :
+  forall e1 e2 : arithmetic_expression,
+    evaluate_ltr (Plus e1 e2) =
+    match evaluate_ltr e1 with
+    | Expressible_nat n1 =>
+      match evaluate_ltr e2 with
+      | Expressible_nat n2 =>
+        Expressible_nat (n1 + n2)
+      end
+    end.
+Proof.
+  fold_unfold_tactic evaluate_ltr.
+Qed.
+
+Lemma fold_unfold_evaluate_ltr_Times :
+  forall e1 e2 : arithmetic_expression,
+    evaluate_ltr (Times e1 e2) =
+    match evaluate_ltr e1 with
+    | Expressible_nat n1 =>
+      match evaluate_ltr e2 with
+      | Expressible_nat n2 =>
+        Expressible_nat (n1 * n2)
+      end
+    end.
+Proof.
+  fold_unfold_tactic evaluate_ltr.
+Qed.
+
+(* ********** *)
+
+Definition test_simplifier (candidate : arithmetic_expression -> arithmetic_expression) :=
+  let ae1 := Plus (Literal 1) (Literal 0) in
+  let ae2 := Plus (Literal 0) (Literal 1) in
+  let ae3 := Times (Literal 1) (Literal 2) in
+  let ae4 := Times (Literal 2) (Literal 1) in
+  let ae5 := Times (Literal 2) (Literal 0) in
+  let ae6 := Times (Literal 0) (Literal 2) in
+  (eqb_arithmetic_expression (candidate ae1) (Literal 1)) &&
+    (eqb_arithmetic_expression (candidate ae2) (Literal 1)) &&
+    (eqb_arithmetic_expression (candidate ae3) (Literal 2)) &&
+    (eqb_arithmetic_expression (candidate ae4) (Literal 2)) &&
+    (eqb_arithmetic_expression (candidate ae5) (Literal 0)) &&
+    (eqb_arithmetic_expression (candidate ae6) (Literal 0))
+.
 
 (* ********** *)
 
